src/coq/Semantics/InterpretationStack.v
@@ -28,8 +28,7 @@ From Vellvm.Handlers Require Export
 
 (* end hide *)
 
-Module Type InterpreterStack.
-  Declare Module LP : LLVMParams.
+Module Type InterpreterStack_common (LP : LLVMParams).
   Module LLVM := Lang.Make LP.
 
   Export LLVM.Events.
@@ -187,8 +186,17 @@ Module Type InterpreterStack.
     Ltac intros3 := intros (? & ? & ? & ?).
 
   End SemNotations.
+End InterpreterStack_common.
+
+Module Type InterpreterStack.
+  Declare Module LP : LLVMParams.
+  Include InterpreterStack_common LP.
 End InterpreterStack.
 
+Module Type InterpreterStackBig <: InterpreterStack.
+  Declare Module LP : LLVMParamsBig.
+  Include InterpreterStack_common LP.
+End InterpreterStackBig.
 
 Module Make (LP' : LLVMParams) : InterpreterStack.
   Module LP := LP'.
@@ -352,5 +360,167 @@ Module Make (LP' : LLVMParams) : InterpreterStack.
   End SemNotations.
 End Make.
 
-Module InterpreterStackBigIntptr := Make LLVMParamsBigIntptr.
+Module MakeBig (LP' : LLVMParamsBig) : InterpreterStackBig.
+  Module LP := LP'.
+  Export LP.
+
+  Module LLVM := Lang.Make LP.
+
+  Export LLVM.Events.
+  Export LLVM.Intrinsics.
+  Export LLVM.MEM.
+  Export LLVM.Pick.
+  Export LLVM.Global.
+  Export LLVM.Local.
+  Export LLVM.Stack.
+  Export LLVM.D.
+  
+  Section InterpreterMCFG.
+
+    (**
+   Partial interpretations of the trees produced by the denotation of _VIR_ programs.
+   The intent is to allow us to only interpret as many layers as needed
+   to perform the required semantic reasoning, and lift for free the
+   equivalence down the pipe.
+   This gives us a _vertical_ notion of compositionality.
+     *)
+
+    Definition interp_mcfg1 {R} (t: itree L0 R) g : itree L1 (global_env * R) :=
+      let uvalue_trace       := interp_intrinsics t in
+      let L1_trace           := interp_global uvalue_trace g in
+      L1_trace.
+
+    Definition interp_mcfg2 {R} (t: itree L0 R) g l : itree L2 (local_env * stack * (global_env * R)) :=
+      let uvalue_trace   := interp_intrinsics t in
+      let L1_trace       := interp_global uvalue_trace g in
+      let L2_trace       := interp_local_stack L1_trace l in
+      L2_trace.
+
+    Definition interp_mcfg3 {R} (t: itree L0 R) g l m : itree L3 (MemState * (local_env * stack * (global_env * R))) :=
+      let uvalue_trace   := interp_intrinsics t in
+      let L1_trace       := interp_global uvalue_trace g in
+      let L2_trace       := interp_local_stack L1_trace l in
+      let L3_trace       := interp_memory L2_trace m in
+      L3_trace.
+
+    Definition interp_mcfg4 {R} RR (t: itree L0 R) g l m : PropT L4 (MemState * (local_env * stack * (global_env * R))) :=
+      let uvalue_trace   := interp_intrinsics t in
+      let L1_trace       := interp_global uvalue_trace g in
+      let L2_trace       := interp_local_stack L1_trace l in
+      let L3_trace       := interp_memory L2_trace m in
+      let L4_trace       := model_undef RR L3_trace in
+      L4_trace.
+
+    (* The interpreter stray away from the model starting from the fourth layer: we pick an arbitrary valid path of execution *)
+    Definition interp_mcfg4_exec {R} (t: itree L0 R) g l m : itree L4 (MemState * (local_env * stack * (global_env * R))) :=
+      let uvalue_trace   := interp_intrinsics t in
+      let L1_trace       := interp_global uvalue_trace g in
+      let L2_trace       := interp_local_stack L1_trace l in
+      let L3_trace       := interp_memory L2_trace m in
+      let L4_trace       := exec_undef L3_trace in
+      L4_trace.
+
+  End InterpreterMCFG.
+
+  Section InterpreterCFG.
+
+    (**
+   Partial interpretations of the trees produced by the
+   denotation of cfg. They differ from the ones of Vellvm programs by
+   their event signature, as well as by the lack of a stack of local event.
+   The intent is to allow us to only interpret as many layers as needed
+   to perform the required semantic reasoning, and lift for free the
+   equivalence down the pipe.
+   This gives us a _vertical_ notion of compositionality.
+     *)
+
+    (**
+   NOTE: Can we avoid this duplication w.r.t. [interpi]?
+     *)
+
+    Definition interp_cfg1 {R} (t: itree instr_E R) (g: global_env) : itree (CallE +' IntrinsicE +' LLVMEnvE +' MemoryE +' PickE +' OOME +' UBE +' DebugE +' FailureE) (global_env * R) :=
+      let L0_trace       := interp_intrinsics t in
+      let L1_trace       := interp_global L0_trace g in
+      L1_trace.
+
+    Definition interp_cfg2 {R} (t: itree instr_E R) (g: global_env) (l: local_env) : itree (CallE +' IntrinsicE +' MemoryE +' PickE +' OOME +' UBE +' DebugE +' FailureE) (local_env * (global_env * R)) :=
+      let L0_trace       := interp_intrinsics t in
+      let L1_trace       := interp_global L0_trace g in
+      let L2_trace       := interp_local L1_trace l in
+      L2_trace.
+
+    Definition interp_cfg3 {R} (t: itree instr_E R) (g: global_env) (l: local_env) (m: MemState) : itree (CallE +' PickE +' OOME +' UBE +' DebugE +' FailureE) (MemState * (local_env * (global_env * R))) :=
+      let L0_trace       := interp_intrinsics t in
+      let L1_trace       := interp_global L0_trace g in
+      let L2_trace       := interp_local L1_trace l in
+      let L3_trace       := interp_memory L2_trace m in
+      L3_trace.
+
+    Definition interp_cfg4 {R} RR (t: itree instr_E R) (g: global_env) (l: local_env) (m: MemState) : PropT (CallE +' OOME +' UBE +' DebugE +' FailureE) (MemState * (local_env * (global_env * R))) :=
+      let L0_trace       := interp_intrinsics t in
+      let L1_trace       := interp_global L0_trace g in
+      let L2_trace       := interp_local L1_trace l in
+      let L3_trace       := interp_memory L2_trace m in
+      let L4_trace       := model_undef RR L3_trace in
+      L4_trace.
+
+  End InterpreterCFG.
+
+  Module SemNotations.
+
+    Notation ℑ1 := interp_cfg1.
+    Notation ℑ2 := interp_cfg2.
+    Notation ℑ3 := interp_cfg3.
+    Notation ℑ4 := interp_cfg4.
+    Notation ℑ  := interp_cfg4.
+
+    Notation ℑs1 := interp_mcfg1.
+    Notation ℑs2 := interp_mcfg2.
+    Notation ℑs3 := interp_mcfg3.
+    Notation ℑs4 := interp_mcfg4.
+    Notation ℑs  := interp_mcfg4.
+
+    Notation Ret1 g x     := (Ret (g,x)).
+    Notation Ret2 g l x   := (Ret (l,(g,x))).
+    Notation Ret3 g l m x := (Ret (m,(l,(g,x)))).
+
+    Notation "⟦ e 'at?' t '⟧e'" :=  (denote_exp t e).
+    Notation "⟦ e 'at' t '⟧e'" :=   (denote_exp (Some t) e).
+    Notation "⟦ e '⟧e'" :=          (denote_exp None e).
+    Notation "⟦ e 'at?' t '⟧e3'" := (ℑ3 (translate exp_to_instr ⟦ e at? t ⟧e)).
+    Notation "⟦ e 'at' t '⟧e3'" :=  (ℑ3 (translate exp_to_instr ⟦ e at t ⟧e)).
+    Notation "⟦ e '⟧e3'" :=         (ℑ3 (translate exp_to_instr ⟦ e ⟧e )).
+
+    Notation "⟦ i '⟧i'" :=        (denote_instr i).
+    Notation "⟦ i '⟧i3'" :=       (ℑ3 ⟦ i ⟧i).
+
+    Notation "⟦ c '⟧c'" :=          (denote_code c).
+    Notation "⟦ c '⟧c3'" :=         (ℑ3 ⟦ c ⟧c).
+
+    Notation "⟦ t '⟧t'" :=        (denote_terminator t).
+    Notation "⟦ t '⟧t3'" :=       (ℑ3 (translate exp_to_instr ⟦ t ⟧t)).
+
+    Notation "⟦ phi '⟧Φ' from"  := (denote_phi from phi) (at level 0, from at next level).
+    Notation "⟦ phi '⟧Φ3' from" := (ℑ3 (denote_phi from phi)) (at level 0, from at next level).
+
+    Notation "⟦ phis '⟧Φs' from"  := (denote_phis from phis) (at level 0, from at next level).
+    Notation "⟦ phis '⟧Φs3' from" := (ℑ3 (denote_phis from phis)) (at level 0, from at next level).
+
+    Notation "⟦ bk '⟧b'" :=  (denote_block bk).
+    Notation "⟦ bk '⟧b3' id" := (ℑ3 (⟦ bk ⟧b id)) (at level 0, id at next level).
+
+    Notation "⟦ bks '⟧bs'"  := (denote_ocfg bks).
+    Notation "⟦ bks '⟧bs3' ids" := (ℑ3 (denote_ocfg bks ids)) (at level 0, ids at next level).
+
+    Notation "⟦ f '⟧cfg'"  := (denote_cfg f).
+    Notation "⟦ f '⟧cfg3'" := (ℑ3 (denote_cfg f)).
+
+    Notation "⟦ f '⟧f'"  := (denote_function f).
+
+    Ltac intros3 := intros (? & ? & ? & ?).
+
+  End SemNotations.
+End MakeBig.
+
+Module InterpreterStackBigIntptr := MakeBig LLVMParamsBigIntptr.
 Module InterpreterStack64BitIntptr := Make LLVMParams64BitIntptr.
