src/coq/Semantics/LLVMParams.v
@@ -12,6 +12,18 @@ Module Type LLVMParams.
   Declare Module ITOP : ITOP ADDR PROV.
 End LLVMParams.
 
+Module Type LLVMParamsBig <: LLVMParams.
+  Declare Module ADDR : ADDRESS.
+  Declare Module IP : INTPTR.
+  Declare Module SIZEOF : Sizeof.
+  Declare Module PTOI : PTOI ADDR.
+  Declare Module PROV : PROVENANCE ADDR.
+  Declare Module ITOP : ITOP ADDR PROV.
+
+  (* Additional module *)
+  Declare Module IP_BIG : INTPTR_BIG IP.
+End LLVMParamsBig.  
+
 Module Make (ADDR' : ADDRESS) (IP' : INTPTR) (SIZEOF' : Sizeof) (PTOI' : PTOI ADDR') (PROV' : PROVENANCE ADDR') (ITOP' : ITOP ADDR' PROV') : LLVMParams.
   Module ADDR := ADDR'.
   Module IP := IP'.
@@ -20,3 +32,13 @@ Module Make (ADDR' : ADDRESS) (IP' : INTPTR) (SIZEOF' : Sizeof) (PTOI' : PTOI AD
   Module PROV := PROV'.
   Module ITOP := ITOP'.
 End Make.
+
+Module MakeBig (ADDR' : ADDRESS) (IP' : INTPTR) (SIZEOF' : Sizeof) (PTOI' : PTOI ADDR') (PROV' : PROVENANCE ADDR') (ITOP' : ITOP ADDR' PROV') (IP_BIG' : INTPTR_BIG IP') : LLVMParamsBig.
+  Module ADDR := ADDR'.
+  Module IP := IP'.
+  Module SIZEOF := SIZEOF'.
+  Module PTOI := PTOI'.
+  Module PROV := PROV'.
+  Module ITOP := ITOP'.
+  Module IP_BIG := IP_BIG'.
+End MakeBig.
